pulse/lib/steel/Steel.Memory.fsti
@@ -511,6 +511,13 @@ let add_inv (#p:slprop) (e:inames) (i:inv p) : inames =
   Set.union (Set.singleton (name_of_inv i)) (reveal e)
 
 (** Creates a new invariant from a separation logic predicate [p] owned at the time of the call *)
+let fresh_wrt (ctx:list (q:_ & inv q))
+              (i:iname)
+  = forall qi'. List.Tot.memP qi' ctx ==> name_of_inv (dsnd qi') <> i
+
+val fresh_invariant (e:inames) (p:slprop) (ctx:list (q:_ & inv q))
+  : action_except (i:inv p { not (mem_inv e i) /\ fresh_wrt ctx (name_of_inv i) }) e p (fun _ -> emp)
+
 val new_invariant (e:inames) (p:slprop)
   : action_except (inv p) e p (fun _ -> emp)
 
@@ -611,42 +618,3 @@ val star_is_witinv_right (#a:Type)
   : Lemma (requires (is_witness_invariant g))
           (ensures  (is_witness_invariant (fun x -> f x `star` g x)))
           //[SMTPat   (is_witness_invariant (fun x -> f x `star` g x))]
-
-// An alternate version of invariant masks
-val owns_invariants_in (e:inames) (m:mem u#a) : slprop u#a
-
-effect UsingInvariants
-  (a:Type u#a)
-  (invariants:inames)
-  (expects:slprop u#1)
-  (provides: a -> slprop u#1)
-  (frame:slprop u#1)
-  = NMSTTotal.NMSTATETOT a (full_mem u#1) mem_evolves
-    (requires fun m0 ->
-        inames_ok invariants m0 /\
-        interp (expects `star` frame `star` owns_invariants_in invariants m0) m0)
-    (ensures fun m0 x m1 ->
-        inames_ok invariants m1 /\
-        interp (expects `star` frame `star` owns_invariants_in invariants m0) m0 /\  //TODO: fix the effect so as not to repeat this
-        interp (provides x `star` frame `star` owns_invariants_in invariants m1) m1)
-
-val flush : unit
-(** An action is just a thunked computation in [MstTot] that takes a frame as argument *)
-let action_using (a:Type u#a) (invariants:inames) (expects:slprop) (provides: a -> slprop) =
-  frame:slprop -> UsingInvariants a invariants expects provides frame
-
-val alloc_invariant (fresh:list (p:_ & inv p)) (e:inames) (p:slprop)
-  : action_using
-    (i:inv p {
-        forall j. j `List.Tot.memP` fresh ==>
-                  name_of_inv i =!= name_of_inv (dsnd j)
-    }) e p (fun _ -> emp)
-
-val use_invariant (#a:Type)
-                  (#fp:slprop)
-                  (#fp':a -> slprop)
-                  (#uses:inames)
-                  (#p:slprop)
-                  (i:inv p{not (mem_inv uses i)})
-                  (f:action_using a uses (p `star` fp) (fun x -> p `star` fp' x))
-  : action_except a (add_inv uses i) fp fp'
